DS/BTree.v
@@ -16,73 +16,7 @@ Inductive BTree (A : Type) : Type :=
 Arguments empty {A}.
 Arguments node {A} _ _ _.
 
-Fixpoint size {A : Type} (bt : BTree A) : nat :=
-match bt with
-    | empty => 0
-    | node _ l r => S (size l + size r)
-end.
-
-Lemma size_swap :
-  forall (A : Type) (v : A) (l r : BTree A),
-    size (node v l r) = size (node v r l).
-Proof.
-  intros. cbn. rewrite plus_comm. trivial.
-Qed.
-
-Definition root {A : Type} (bt : BTree A) : option A :=
-match bt with
-    | empty => None
-    | node v l r => Some v
-end.
-
-Fixpoint map {A B : Type} (f : A -> B) (bt : BTree A) : BTree B :=
-match bt with
-    | empty => empty
-    | node v l r => node (f v) (map f l) (map f r)
-end.
-
-(*From mathcomp Require Import ssreflect.*)
-
-Theorem map_pres_size : forall (A B : Type) (f : A -> B) (bt : BTree A),
-    size bt = size (map f bt).
-Proof.
-  induction bt as [| v l Hl r Hr]; cbn; intros;
-  rewrite <- ?Hl, <- ?Hr; reflexivity.
-(*Restart.
-  intros. elim: bt => //= v l -> r -> //=. *)
-Qed.
-
-Fixpoint combine
-  {A B : Type} (ta : BTree A) (tb : BTree B) : BTree (A * B) :=
-match ta, tb with
-    | empty, _ => empty
-    | _, empty => empty
-    | node v1 l1 r1, node v2 l2 r2 =>
-        node (v1, v2) (combine l1 l2) (combine r1 r2)
-end.
-
-Fixpoint fold
-  {A B : Set} (op : A -> B -> B -> B) (b : B) (bt : BTree A) : B :=
-match bt with
-    | empty => b
-    | node v l r => op v (fold op b l) (fold op b r)
-end.
-
-Definition bool_to_nat (b : bool) : nat :=
-match b with
-    | true => 1
-    | false => 0
-end.
-
-Definition size_fold {A : Set} := @fold A nat (fun _ l r => 1 + l + r) 0.
-Definition sum_fold := fold (fun v l r => v + l + r) 0.
-Definition find_fold (n : nat) : BTree nat -> bool :=
-    fold (fun v l r => orb (beq_nat v n) (orb l r)) false.
-Definition count_fold (n : nat) : BTree nat -> nat :=
-    fold (fun v l r => bool_to_nat (beq_nat v n) + l + r) 0.
-Definition map_fold {A B : Set} (f : A -> B) : BTree A -> BTree B :=
-    fold (fun v l r => node (f v) l r) empty.
-
+(** The [elem] predicate. *)
 Inductive elem {A : Type} (a : A) : BTree A -> Prop :=
     | elem_root : forall l r : BTree A, elem a (node a l r)
     | elem_left : forall (v : A) (l r : BTree A),
@@ -92,95 +26,90 @@ Inductive elem {A : Type} (a : A) : BTree A -> Prop :=
 
 Hint Constructors elem.
 
-Theorem elem_dec :
+(*Theorem elem_dec :
   forall {A : Type} {dec : EqDec A eq} (a : A) (t : BTree A),
     {elem a t} + {~ elem a t}.
 Proof.
-  induction t as [| v l IHl r IHr].
-    right. inversion 1.
+  induction t as [| v l [IHl | IHl] r [IHr | IHr]]; auto.
+    right. inv 1.
     destruct (dec a v).
-      left. rewrite <- e. constructor.
-      destruct IHl as [IHl1 | IHl2].
-        left. apply elem_left. assumption.
-        destruct IHr as [IHr1 | IHr2].
-          left. apply elem_right; assumption.
-          right. intro. inversion H; contradiction.
-(*Restart.
-  intros. elim: t => [| v l [Hl | Hl] r [Hr | Hr]]; auto.
-    right. inversion 1.
-    case: (dec a v) => H; [left | right].
-      by rewrite H.
-      by inversion 1.*)
-Defined.
+      left. rewrite  e. auto.
+      right. inv 1.
+Defined.*)
 
 Fixpoint elem_decb
-  {A : Type} (dec : EqDec A eq) (x : A) (t : BTree A) : bool :=
+  {A : LinDec} (x : A) (t : BTree A) : bool :=
 match t with
     | empty => false
     | node v l r =>
-        if dec x v
-        then true
-        else elem_decb dec x l || elem_decb dec x r
+        (x =? v) || elem_decb x l || elem_decb x r
 end.
 
-Require Import Bool.
+Definition root {A : Type} (bt : BTree A) : option A :=
+match bt with
+    | empty => None
+    | node v l r => Some v
+end.
 
-Lemma elem_decb_reflect :
-  forall (A : Type) (dec : EqDec A eq) (x : A) (t : BTree A),
-    reflect (elem x t) (elem_decb dec x t).
-Proof.
-  induction t as [| v l IHl r IHr]; cbn.
-    constructor. inversion 1.
-    destruct (dec x v), IHl, IHr; try inv e; cbn; auto.
-      constructor. intro. inv H. contradiction c. reflexivity.
-Qed.
-
-(* toList, fromList and their variants *)
+(* [BTree_toList], [fromList] and their variants *)
 Function BTree_toList {A : Type} (t : BTree A) : list A :=
 match t with
     | empty => []
     | node v l r => BTree_toList l ++ v :: BTree_toList r
 end.
 
-Function toList'_aux {A : LinDec} (t : BTree A) (acc : list A) : list A :=
+Function BTree_toList'_aux {A : LinDec} (t : BTree A) (acc : list A) : list A :=
 match t with
     | empty => acc
-    | node v l r => toList'_aux l (v :: toList'_aux r acc)
+    | node v l r => BTree_toList'_aux l (v :: BTree_toList'_aux r acc)
 end.
 
-Definition toList' {A : LinDec} (t : BTree A) : list A :=
-  toList'_aux t [].
+Definition BTree_toList' {A : LinDec} (t : BTree A) : list A :=
+  BTree_toList'_aux t [].
 
-Lemma toList'_aux_spec :
-  forall (A : LinDec) (t : BTree A) (acc : list A),
-    toList'_aux t acc = BTree_toList t ++ acc.
+(** [size] and counting. *)
+Fixpoint size {A : Type} (bt : BTree A) : nat :=
+match bt with
+    | empty => 0
+    | node _ l r => S (size l + size r)
+end.
+
+Fixpoint count_BTree {A : LinDec} (x : A) (t : BTree A) : nat :=
+match t with
+    | empty => 0
+    | node v l r =>
+        let n := count_BTree x l in
+        let m := count_BTree x r in
+        if x =? v then S (n + m) else n + m
+end.
+
+(** Propertes of [elem] and [elem_decb]. *)
+
+Lemma elem_decb_reflect :
+  forall (A : LinDec) (x : A) (t : BTree A),
+    reflect (elem x t) (elem_decb x t).
 Proof.
-  intros. functional induction @toList'_aux A t acc; cbn.
+  induction t as [| v l IHl r IHr]; cbn.
+    constructor. inv 1.
+    dec. destruct IHl, IHr; auto.
+      constructor. inv 1.
+Qed.
+
+(** Properties of casts to/from list. *)
+
+Lemma BTree_toList'_aux_spec :
+  forall (A : LinDec) (t : BTree A) (acc : list A),
+    BTree_toList'_aux t acc = BTree_toList t ++ acc.
+Proof.
+  intros. functional induction @BTree_toList'_aux A t acc; cbn.
     trivial.
     rewrite <- app_assoc. cbn. rewrite <- IHl, <- IHl0. trivial.
 Qed.
 
-Theorem toList'_spec : @toList' = @BTree_toList.
+Theorem BTree_toList'_spec : @BTree_toList' = @BTree_toList.
 Proof.
-  ext A. ext t. unfold toList'.
-  rewrite toList'_aux_spec, app_nil_r. trivial.
-Qed.
-
-(* Counting elements in a binary tree. *)
-Fixpoint count_BTree (A : LinDec) (x : A) (t : BTree A) : nat :=
-match t with
-    | empty => 0
-    | node v l r =>
-        let n := count_BTree A x l in
-        let m := count_BTree A x r in
-        if x =? v then S (n + m) else n + m
-end.
-
-Lemma count_toList :
-  forall (A : LinDec) (x : A) (t : BTree A),
-    count A x (BTree_toList t) = count_BTree A x t.
-Proof.
-  induction t; cbn; rewrite ?count_app; dec.
+  ext A. ext t. unfold BTree_toList'.
+  rewrite BTree_toList'_aux_spec, app_nil_r. trivial.
 Qed.
 
 Lemma toList_In_elem :
@@ -191,4 +120,29 @@ Proof.
     induction t; cbn; intros; try apply in_app_or in H; firstorder.
       subst. firstorder.
     induction 1; cbn; firstorder.
+Qed.
+
+(** Properties of [size]. *)
+
+Lemma size_swap :
+  forall (A : Type) (v : A) (l r : BTree A),
+    size (node v l r) = size (node v r l).
+Proof.
+  intros. cbn. rewrite plus_comm. trivial.
+Qed.
+
+Lemma size_length :
+  forall (A : Type) (t : BTree A),
+    length (BTree_toList t) = size t.
+Proof.
+  induction t; cbn.
+    reflexivity.
+    rewrite !app_length. cbn. rewrite IHt1, IHt2. omega.
+Qed.
+
+Lemma count_toList :
+  forall (A : LinDec) (x : A) (t : BTree A),
+    count A x (BTree_toList t) = count_BTree x t.
+Proof.
+  induction t; cbn; rewrite ?count_app; dec.
 Qed.
