Sorting/TrichQuicksortSpec.v
@@ -31,6 +31,42 @@ Proof.
   intros. rewrite !count_In, <- htqs_perm; auto. reflexivity.
 Qed.
 
+Lemma list_ind2 :
+  forall (A : Type) (P : list A -> Prop),
+    P [] -> (forall x : A, P [x]) ->
+    (forall (h1 h2 : A) (t : list A), P t -> P (h1 :: h2 :: t)) ->
+      forall l : list A, P l.
+Proof.
+  fix 6. destruct l as [| h1 [| h2 t]]; auto.
+  apply H1. apply list_ind2; auto.
+Qed.
+
+Lemma filter_eqb_repeat :
+  forall (A : LinDec) (x : A) (l : list A),
+    exists n : nat, filter (fun x' : A => x' =? x) l = repeat x n.
+Proof.
+  induction l as [| h t]; cbn.
+    exists 0. reflexivity.
+    dec. destruct IHt as [n H]. exists (S n). cbn. rewrite H. reflexivity.
+Qed.
+
+Lemma repeat_sorted :
+  forall (A : LinDec) (x : A) (n : nat),
+    sorted A (repeat x n).
+Proof.
+  induction n as [| n']; cbn.
+    constructor.
+    destruct n'; cbn; constructor; auto.
+Qed.
+
+Lemma filter_eqb_sorted :
+  forall (A : LinDec) (x : A) (l : list A),
+    sorted A (filter (fun x' : A => x' =? x) l).
+Proof.
+  intros. destruct (filter_eqb_repeat A x l) as [n H].
+  rewrite H. apply repeat_sorted.
+Qed.
+
 Theorem htqs_sorted :
   forall (n : nat) (A : TrichDec) (s : Sort) (l : list A),
     sorted A (htqs n A sort l).
@@ -45,16 +81,23 @@ Proof.
           rewrite htqs_In, filter_In in H. destruct H.
             unfold TrichDec_ltb in H0. case_eq (h <?> x); intro;
             rewrite H1 in H0; trich.
-        Search ((_, _) = (_, _)).
-        destruct (filter
-          (fun x : @carrier A => @LinDec_eqb (TrichDec_to_LinDec A) x h) t).
-          cbn. assumption.
-          cbn.
-Admitted. (* TODO *)
+        apply sorted_app; auto.
+          apply filter_eqb_sorted.
+          intros. rewrite filter_In in H. destruct H. eapply perm_In in H0.
+            Focus 2. rewrite <- htqs_perm. reflexivity.
+            apply filter_In in H0. destruct H0.
+              unfold TrichDec_ltb in H2; case_eq (h <?> y); intro;
+                rewrite H3 in H2; trich.
+      intros. eapply perm_In in H.
+        Focus 2. rewrite <- htqs_perm. reflexivity.
+        apply filter_In in H. destruct H.
+          unfold TrichDec_ltb in H0; case_eq (x <?> h); intro;
+          rewrite H1 in H0; trich.
+Qed.
 
-(* TODO Instance Sort_htqs (n : nat) (s : Sort) : Sort :=
+(*Instance Sort_htqs (n : nat) (s : Sort) : Sort :=
 {
-    TODO sort := fun A : TrichDec => htqs n A (@sort s A)
+    sort := fun A : TrichDec => htqs n A (@sort s A)
 }.
 Proof.
   intros. apply htqs_sorted.
